add linear cells; progress on RwLock acquire

concurrency/framework/Cells.s.dfy
@@ -1,3 +1,5 @@
+include "../../lib/Base/Option.s.dfy"
+
 module {:extern "Cells"} Cells {
   type {:extern "struct"} Cell(!new,00)<V>
   datatype CellContents<V> = CellContents(ghost cell: Cell<V>, v: V)
@@ -14,4 +16,36 @@ module {:extern "Cells"} Cells {
   method {:extern} write_cell<V>(shared cell: Cell<V>, glinear inout cellContents: CellContents<V>, v: V)
   requires cell == old_cellContents.cell
   ensures cellContents == old_cellContents.(v := v)
+}
+
+module {:extern "LinearCells"} LinearCells {
+  import opened Options
+
+  type {:extern "struct"} LinearCell(!new,00)<V>
+  datatype CellContents<V> = CellContents(ghost lcell: LinearCell<V>, v: Option<V>)
+
+  method {:extern} new_cell<V>()
+  returns (linear lcell: LinearCell<V>, glinear cellContents: CellContents<V>)
+  ensures cellContents == CellContents(lcell, None)
+
+  method {:extern} read_lcell<V>(shared lcell: LinearCell<V>, gshared cellContents: CellContents<V>)
+  returns (shared v: V)
+  requires cellContents.lcell == lcell
+  requires cellContents.v.Some?
+  ensures cellContents.v.value == v
+
+  method {:extern} take_lcell<V>(shared lcell: LinearCell<V>, glinear cellContents: CellContents<V>)
+  returns (linear v: V, glinear cellContents': CellContents<V>)
+  requires cellContents.lcell == lcell
+  requires cellContents.v.Some?
+  ensures cellContents.v.value == v
+  ensures cellContents'.lcell == lcell
+  ensures cellContents'.v == None
+
+  method {:extern} give_lcell<V>(shared lcell: LinearCell<V>, glinear cellContents: CellContents<V>, linear v: V)
+  returns (glinear cellContents': CellContents<V>)
+  requires cellContents.lcell == lcell
+  requires cellContents.v.None?
+  ensures cellContents'.lcell == lcell
+  ensures cellContents'.v == Some(v)
 }
